Some changes

theories/Example.v
@@ -2,10 +2,527 @@
 
 From MailboxTypes Require Import TypingRules.
 From MailboxTypes Require Import Util.
+From MailboxTypes Require Import Substitution.
 
 From Stdlib Require Import Lists.List.
 Import ListNotations.
 
+
+(*
+  def client() : 1 {
+    let server = new in
+    spawn server_listen(server);
+    let self = new in
+    server!Ping[self];
+    guard self : _ {
+      receive Pong[r] from self |-> free self; ()
+    }
+  }
+
+   def server_listen(self) : 1 {
+      guard self : Ping {
+        receive Ping[reply] from self |->
+          reply!Pong[sefl];
+          free self; ()
+      }
+   }
+
+  M ; N = let x : 1 = M in N = TLet M N
+  => M ;; N
+
+
+  def client() : 1 {
+    let server = new in
+    let spawn server_listen(server) in
+    let self = new in
+    let server!Ping[self] in
+    guard self : _ {
+      receive Pong[r] from self |-> free self; ()
+    }
+  }
+*)
+
+Infix ";;" := TLet (at level 66, left associativity).
+
+Section ping_pong_example.
+
+  Inductive PingPong : Type :=
+    | Ping
+    | Pong.
+
+  Instance PingPongMessage : IMessage PingPong.
+  Proof.
+    constructor.
+    - destruct m, n; now (left + right).
+    - apply (fun _ => 1).
+  Defined.
+
+  Definition sig (m : PingPong) :=
+    match m with
+    | Ping => TTMailbox(! « Pong »)
+    | Pong => TTBase BTUnit
+    end.
+
+  Inductive PingPongDefinition : Type :=
+    | Client
+    | ServerListen.
+
+  Instance PingPongDefinitionName : IDefinitionName PingPongDefinition.
+  Proof.
+    constructor; destruct m; destruct n; now (left + right).
+  Defined.
+
+  (*Definition Client_body : Term :=*)
+  (*  TNew ;; (TSpawn (TApp ServerListen (ValueVar 0))) ;;*)
+  (*  TNew ;; (TSend (ValueVar 2) Ping (ValueVar 0)) ;;*)
+  (*  TGuard (ValueVar 1) « Pong » [*)
+  (*    GReceive Pong (TGuard (ValueVar 1) 𝟙 [GFree (TValue ValueUnit)])*)
+  (*  ].*)
+
+  Definition Client_body : Term :=
+    TLet
+      TNew
+      (TLet (TSpawn (TApp ServerListen (ValueVar 0)))
+        (TLet TNew
+          (TLet (TSend (ValueVar 2) Ping (ValueVar 0))
+            (TGuard (ValueVar 1) « Pong » [
+                GReceive Pong (TGuard (ValueVar 1) 𝟙 [GFree (TValue ValueUnit)])
+              ])
+      ))).
+
+  Lemma asdfe : subst (ValueUnit) 0 Client_body = Client_body.
+  Proof.
+    unfold Client_body.
+    simpl_subst_goal; simpl.
+    simpl_lift_goal; simpl.
+    simpl_subst_goal. reflexivity.
+  Qed.
+
+  Compute lift 3 4 (ValueVar 3).
+  Compute lift 2 1 (TLet (TValue ValueUnit) (TValue (ValueVar 1))).
+  Compute subst (ValueUnit) 3 Client_body.
+  Compute lift 0 4 Client_body.
+
+  Definition ServerListen_body : Term :=
+    TGuard (ValueVar 0) (« Ping » ⊕ 𝟙) [
+      GReceive Ping (TLet (TSend (ValueVar 0) Pong (ValueUnit)) (TGuard (ValueVar 2) 𝟙 [GFree (TValue ValueUnit)]));
+      GFree (TValue ValueUnit)
+    ].
+
+  (* TODO: Check if it makes sense for 0 arguments to be represented by unit type *)
+  Definition ClientDefinition : FunctionDefinition :=
+    FunDef Client (TUBase BTUnit) (TUBase BTUnit) Client_body.
+
+  (* We use ⋆ « Ping »*)
+  Definition ServerListenDefinition : FunctionDefinition :=
+    FunDef ServerListen (? « Ping » ⊕ 𝟙 ^^ •) (TUBase BTUnit) ServerListen_body.
+
+  Definition PingPongDefinitions (d : PingPongDefinition) :=
+    match d with
+    | Client => ClientDefinition
+    | ServerListen => ServerListenDefinition
+    end.
+
+  Definition PingPongProgram :=
+    {|
+      signature := sig
+    ; definitions := PingPongDefinitions
+    ; initialTerm := Client_body
+    |}.
+
+  Lemma ServerListen_WellTyped : WellTypedDefinition PingPongProgram ServerListenDefinition.
+  Proof.
+    constructor.
+    unfold ServerListen_body.
+    eapply GUARD with (env1 := [Some (? « Ping » ⊕ 𝟙 ^^ •)]) (env2 := [None]) (f := (« Ping » ⊙ 𝟙) ⊕ 𝟙).
+    - repeat constructor.
+    - eapply SUB with (T1 := (? « Ping » ⊕ 𝟙^^ •)) (env2 := [Some (? « Ping » ⊕ 𝟙 ^^ •)]).
+      + apply EnvironmentSubtype_refl.
+      + constructor.
+        * intros m mIn.
+          inversion mIn; subst.
+          apply MPValueChoiceLeft.
+          now apply MPComp_MPInclusion_One.
+          now apply MPValueChoiceRight.
+        * constructor.
+      + rewrite <- raw_insert_zero.
+        repeat constructor.
+    - constructor.
+      + econstructor.
+        * simpl; reflexivity.
+        * now right.
+        * eapply LET with
+            (T1 := TTBase BTUnit)
+            (env1 := (insert 0 (! « Pong » ^^ ◦) [None; None]))
+            (env2 := (insert 1 (? 𝟙 ^^ •) [None; None])).
+          -- repeat rewrite raw_insert_successor.
+             repeat rewrite raw_insert_zero.
+             simpl.
+             rewrite lookup_zero.
+             repeat constructor.
+          -- simpl.
+             eapply SEND with
+               (env1 := insert 0 (! « Pong » ^^ ◦) [None ; None])
+               (env2 := [None; None ; None]).
+             ++ repeat constructor.
+             ++ simpl; reflexivity.
+             ++ repeat rewrite raw_insert_zero; repeat constructor.
+             ++ simpl.
+                constructor; repeat constructor.
+          -- eapply GUARD with
+               (f := 𝟙)
+               (env1 := insert 2 (? 𝟙 ^^ •) [None; None; None])
+               (env2 := insert 0 (TUBase BTUnit) [None; None; None]).
+             ++ repeat rewrite raw_insert_successor.
+               repeat rewrite raw_insert_zero.
+               simpl.
+               repeat rewrite lookup_zero.
+               repeat constructor.
+             ++ repeat constructor.
+             ++ do 2 constructor.
+                eapply SUB with (env2 := repeat None 4).
+                ** simpl; rewrite raw_insert_zero; repeat constructor.
+                ** apply Subtype_refl.
+                ** simpl; repeat constructor.
+             ++ reflexivity.
+             ++ repeat constructor.
+      + repeat constructor.
+    - intros m mIn.
+      inversion mIn; subst.
+      apply MPValueChoiceLeft.
+      now apply MPComp_MPInclusion_One.
+      now apply MPValueChoiceRight.
+    - repeat constructor; econstructor.
+      + repeat constructor.
+      + rewrite MPComp_zero_right.
+        rewrite MPChoice_unit.
+        rewrite MPChoice_unit.
+        now rewrite MPComp_unit.
+  Qed.
+
+  (*Lemma ServerListen_WellTyped : WellTypedDefinition PingPongProgram ServerListenDefinition.*)
+  (*Proof.*)
+  (*  constructor.*)
+  (*  unfold ServerListen_body.*)
+  (*  (*eapply GUARD with (env1 := [Some (? « Ping » ⊕ 𝟙 ^^ •)]) (env2 := [None]) (f := « Ping » ⊙ 𝟙).*)*)
+  (*  eapply GUARD with (env1 := [Some (? « Ping » ⊕ 𝟙 ^^ •)]) (env2 := [None]) (f := (« Ping » ⊕ 𝟙) ⊙ 𝟙).*)
+  (*  - repeat constructor.*)
+  (*  - rewrite <- raw_insert_zero; repeat constructor.*)
+  (*    (*eapply SUB with (T1 := (? « Ping » ^^ •)) (env2 := [Some (? « Ping » ^^ •)]).*)*)
+  (*    (*+ repeat constructor.*)*)
+  (*    (*  intros m mIn.*)*)
+  (*    (*  admit.*)*)
+  (*    (*  (*apply EnvironmentSubtype_refl.*)*)*)
+  (*    (*+ repeat constructor.*)*)
+  (*    (*  apply MPComp_MPInclusion_One.*)*)
+  (*    (*+ rewrite <- raw_insert_zero.*)*)
+  (*    (*  repeat constructor.*)*)
+  (*  - constructor. econstructor.*)
+  (*    + simpl; reflexivity.*)
+  (*    + now right.*)
+  (*    + eapply LET with*)
+  (*        (T1 := TTBase BTUnit)*)
+  (*        (env1 := (insert 0 (! « Pong » ^^ ◦) [None; None]))*)
+  (*        (env2 := (insert 1 (? 𝟙 ^^ •) [None; None])).*)
+  (*      * repeat rewrite raw_insert_successor.*)
+  (*        repeat rewrite raw_insert_zero.*)
+  (*        simpl.*)
+  (*        rewrite lookup_zero.*)
+  (*        repeat constructor.*)
+  (*      * simpl.*)
+  (*        eapply SEND with*)
+  (*          (env1 := insert 0 (! « Pong » ^^ ◦) [None ; None])*)
+  (*          (env2 := [None; None ; None]).*)
+  (*        -- repeat constructor.*)
+  (*        -- simpl; reflexivity.*)
+  (*        -- repeat rewrite raw_insert_zero; repeat constructor.*)
+  (*        -- simpl.*)
+  (*           constructor; repeat constructor.*)
+  (*      * eapply GUARD with*)
+  (*          (f := 𝟙)*)
+  (*          (env1 := insert 2 (? 𝟙 ^^ •) [None; None; None])*)
+  (*          (env2 := insert 0 (TUBase BTUnit) [None; None; None]).*)
+  (*        -- repeat rewrite raw_insert_successor.*)
+  (*           repeat rewrite raw_insert_zero.*)
+  (*           simpl.*)
+  (*           repeat rewrite lookup_zero.*)
+  (*           repeat constructor.*)
+  (*        -- constructor; repeat constructor.*)
+  (*        -- do 2 constructor.*)
+  (*           eapply SUB with (env2 := repeat None 4).*)
+  (*           ++ simpl; rewrite raw_insert_zero; repeat constructor.*)
+  (*           ++ apply Subtype_refl.*)
+  (*           ++ simpl; repeat constructor.*)
+  (*        -- reflexivity.*)
+  (*        -- repeat constructor.*)
+  (*  - apply MPComp_MPInclusion_One.*)
+  (*  - repeat constructor; econstructor.*)
+  (*    + repeat constructor.*)
+  (*    + rewrite MPComp_zero_right.*)
+  (*      rewrite MPChoice_unit.*)
+  (*      now rewrite MPComp_unit.*)
+  (*Qed.*)
+
+  (*Lemma Client_body_WellTyped : WellTypedTerm PingPongProgram [] Client_body (TUBase BTUnit).*)
+  (*Proof.*)
+  (*  unfold Client_body.*)
+  (*  eapply LET with*)
+  (*    (T1 := TTMailbox (? 𝟙))*)
+  (*    (env1 := [])*)
+  (*    (env2 := []).*)
+  (*  - repeat constructor.*)
+  (*  - repeat constructor; reflexivity.*)
+  (*  - simpl.*)
+  (*    eapply LET with*)
+  (*      (T1 := TTBase BTUnit)*)
+  (*      (env1 := [Some (? (« Ping » ⊕ 𝟙) ⊙ 𝟙 ^^ ◦)])*)
+  (*      (env2 := [Some (! (« Ping » ⊕ 𝟙) ^^ •)]).*)
+  (*    + repeat rewrite raw_insert_zero; repeat constructor.*)
+  (*    + apply SPAWN with (env := [Some (? (« Ping » ⊕ 𝟙) ⊙ 𝟙 ^^ •)]).*)
+  (*      * eapply APP; simpl; try reflexivity.*)
+  (*        eapply SUB with (T1 := ? (« Ping » ⊕ 𝟙) ⊙ 𝟙 ^^ •).*)
+  (*        apply EnvironmentSubtype_refl.*)
+  (*        constructor. intros m mIn. now rewrite MPComp_unit in mIn.*)
+  (*        constructor.*)
+  (*        rewrite <- raw_insert_zero; repeat constructor.*)
+  (*      * reflexivity.*)
+  (*    + simpl.*)
+  (*      eapply LET with*)
+  (*        (T1 := TTMailbox (? 𝟙))*)
+  (*        (env1 := [None; None])*)
+  (*        (env2 := insert 0 (TUBase BTUnit) [Some (! « Ping » ⊕ 𝟙 ^^ •)]).*)
+  (*      * repeat rewrite raw_insert_zero; repeat constructor.*)
+  (*      * apply NEW; repeat constructor.*)
+  (*      * simpl.*)
+  (*        eapply LET with*)
+  (*          (T1 := TTBase BTUnit)*)
+  (*          (env1 := [Some (! « Pong » ^^ ◦); Some (TUBase BTUnit); Some (! « Ping » ⊕ 𝟙 ^^ •)])*)
+  (*          (env2 := [Some (? « Pong » ⊙ 𝟙 ^^ •); None; None]).*)
+  (*        -- repeat rewrite raw_insert_zero; repeat constructor.*)
+  (*        -- eapply SEND with*)
+  (*            (env1 := [None; None; Some (! « Ping » ⊕ 𝟙 ^^ •)])*)
+  (*            (env2 := [Some (! « Pong » ^^ ◦); Some (TUBase BTUnit); None]).*)
+  (*          ++ eapply SUB with (env2 := [None; None; Some (! « Ping » ^^ ◦)]).*)
+  (*             ** now repeat constructor.*)
+  (*             ** apply Subtype_refl.*)
+  (*             ** replace [None; None; Some (! « Ping » ^^ ◦)] with (insert 2 (! « Ping » ^^ ◦) [None; None])*)
+  (*                by (repeat rewrite raw_insert_successor; simpl; rewrite lookup_zero; now rewrite raw_insert_zero).*)
+  (*                repeat constructor.*)
+  (*          ++ simpl; reflexivity.*)
+  (*          ++ repeat constructor.*)
+  (*          ++ simpl.*)
+  (*             eapply SUB with (env2 := [Some (! « Pong » ^^ ◦); None; None]).*)
+  (*             ** do 2 constructor; try reflexivity; now repeat constructor.*)
+  (*             ** apply Subtype_refl.*)
+  (*             ** rewrite <- raw_insert_zero; repeat constructor.*)
+  (*        -- eapply SUB with (env2 := [None; Some (? « Pong » ⊙ 𝟙 ^^ •); None; None]).*)
+  (*           ++ rewrite raw_insert_zero; repeat constructor; reflexivity.*)
+  (*           ++ apply Subtype_refl.*)
+  (*           ++ eapply GUARD with*)
+  (*                (env1 := insert 1 (? « Pong » ⊙ 𝟙 ^^ •) [None; None; None])*)
+  (*                (env2 := [None; None; None; None]).*)
+  (*             ** rewrite raw_insert_successor; rewrite raw_insert_zero; rewrite lookup_zero; simpl.*)
+  (*                repeat constructor.*)
+  (*             ** repeat constructor.*)
+  (*             ** constructor.*)
+  (*                eapply RECEIVE.*)
+  (*                --- simpl; reflexivity.*)
+  (*                --- now left.*)
+  (*                --- eapply GUARD with*)
+  (*                      (env1 := insert 1 (? 𝟙 ^^ •) [Some (TUBase BTUnit); None; None; None; None])*)
+  (*                      (env2 := [None; None; None; None; None; None]).*)
+  (*                    +++ rewrite raw_insert_successor.*)
+  (*                        repeat rewrite raw_insert_zero.*)
+  (*                        rewrite lookup_zero; simpl.*)
+  (*                        repeat constructor.*)
+  (*                    +++ eapply SUB with (env2 := insert 1 (? 𝟙 ^^ •) [None; None; None; None; None]).*)
+  (*                        repeat rewrite raw_insert_successor;*)
+  (*                        repeat rewrite raw_insert_zero.*)
+  (*                        repeat rewrite lookup_zero; simpl; repeat constructor; reflexivity.*)
+  (*                        apply Subtype_refl.*)
+  (*                        repeat constructor.*)
+  (*                    +++ repeat constructor.*)
+  (*                    +++ reflexivity.*)
+  (*                    +++ repeat constructor.*)
+  (*             ** apply MPComp_MPInclusion_One.*)
+  (*             ** constructor; econstructor.*)
+  (*                repeat constructor.*)
+  (*                rewrite MPComp_unit.*)
+  (*                rewrite MPComp_zero_right.*)
+  (*                now rewrite MPChoice_unit.*)
+  (*Qed.*)
+
+  Lemma Client_Welltyped : WellTypedDefinition PingPongProgram ClientDefinition.
+  Proof.
+    constructor.
+    unfold Client_body.
+    eapply LET with
+      (T1 := TTMailbox (? 𝟙))
+      (env1 := [Some (TUBase BTUnit)])
+      (env2 := [None]).
+    - repeat constructor.
+    - eapply SUB with (env2 := [None]); repeat constructor; reflexivity.
+    - simpl.
+      eapply LET with
+        (T1 := TTBase BTUnit)
+        (env1 := [Some (? (« Ping » ⊕ 𝟙) ⊙ 𝟙 ^^ ◦); None])
+        (env2 := [Some (! (« Ping » ⊕ 𝟙) ^^ •); None]).
+      + repeat rewrite raw_insert_zero; repeat constructor.
+      + apply SPAWN with (env := [Some (? (« Ping » ⊕ 𝟙) ⊙ 𝟙 ^^ •); None]).
+        * eapply APP; simpl; try reflexivity.
+          eapply SUB with (T1 := ? (« Ping » ⊕ 𝟙) ⊙ 𝟙 ^^ •).
+          apply EnvironmentSubtype_refl.
+          constructor. intros m mIn. now rewrite MPComp_unit in mIn.
+          constructor.
+          rewrite <- raw_insert_zero; repeat constructor.
+        * reflexivity.
+      + simpl.
+        eapply LET with
+          (T1 := TTMailbox (? 𝟙))
+          (env1 := [None; None; None])
+          (env2 := insert 0 (TUBase BTUnit) [Some (! « Ping » ⊕ 𝟙 ^^ •); None]).
+        * repeat rewrite raw_insert_zero; repeat constructor.
+        * apply NEW; repeat constructor.
+        * simpl.
+          eapply LET with
+            (T1 := TTBase BTUnit)
+            (env1 := [Some (! « Pong » ^^ ◦); Some (TUBase BTUnit); Some (! « Ping » ⊕ 𝟙 ^^ •); None])
+            (env2 := [Some (? « Pong » ⊙ 𝟙 ^^ •); None; None; None]).
+          -- repeat rewrite raw_insert_zero; repeat constructor.
+          -- eapply SEND with
+              (env1 := [None; None; Some (! « Ping » ⊕ 𝟙 ^^ •); None])
+              (env2 := [Some (! « Pong » ^^ ◦); Some (TUBase BTUnit); None; None]).
+            ++ eapply SUB with (env2 := [None; None; Some (! « Ping » ^^ ◦); None]).
+               ** now repeat constructor.
+               ** apply Subtype_refl.
+               ** replace [None; None; Some (! « Ping » ^^ ◦); None] with (insert 2 (! « Ping » ^^ ◦) [None; None; None])
+                  by (repeat rewrite raw_insert_successor; simpl; rewrite lookup_zero; now rewrite raw_insert_zero).
+                  repeat constructor.
+            ++ simpl; reflexivity.
+            ++ repeat constructor.
+            ++ simpl.
+               eapply SUB with (env2 := [Some (! « Pong » ^^ ◦); None; None; None]).
+               ** do 2 constructor; try reflexivity; now repeat constructor.
+               ** apply Subtype_refl.
+               ** rewrite <- raw_insert_zero; repeat constructor.
+          -- eapply SUB with (env2 := [None; Some (? « Pong » ⊙ 𝟙 ^^ •); None; None; None]).
+             ++ rewrite raw_insert_zero; repeat constructor; reflexivity.
+             ++ apply Subtype_refl.
+             ++ eapply GUARD with
+                  (env1 := insert 1 (? « Pong » ⊙ 𝟙 ^^ •) [None; None; None; None])
+                  (env2 := [None; None; None; None; None]).
+               ** rewrite raw_insert_successor; rewrite raw_insert_zero; rewrite lookup_zero; simpl.
+                  repeat constructor.
+               ** repeat constructor.
+               ** apply SINGLE.
+                  eapply RECEIVE.
+                  --- simpl; reflexivity.
+                  --- now left.
+                  --- eapply GUARD with
+                        (env1 := insert 1 (? 𝟙 ^^ •) [Some (TUBase BTUnit); None; None; None; None; None])
+                        (env2 := [None; None; None; None; None; None; None]).
+                      +++ rewrite raw_insert_successor.
+                          repeat rewrite raw_insert_zero.
+                          rewrite lookup_zero; simpl.
+                          repeat constructor.
+                      +++ eapply SUB with (env2 := insert 1 (? 𝟙 ^^ •) [None; None; None; None; None; None]).
+                          repeat rewrite raw_insert_successor;
+                          repeat rewrite raw_insert_zero.
+                          repeat rewrite lookup_zero; simpl; repeat constructor; reflexivity.
+                          apply Subtype_refl.
+                          repeat constructor.
+                      +++ repeat constructor.
+                      +++ reflexivity.
+                      +++ repeat constructor.
+               ** apply MPComp_MPInclusion_One.
+               ** constructor; econstructor.
+                  repeat constructor.
+                  rewrite MPComp_unit.
+                  rewrite MPComp_zero_right.
+                  now rewrite MPChoice_unit.
+  Qed.
+
+  Theorem PingPongProgram_WellTyped : WellTypedProgram PingPongProgram.
+  Proof.
+    constructor.
+    - intros [|].
+      + apply Client_Welltyped.
+      + apply ServerListen_WellTyped.
+    - simpl.
+
+End ping_pong_example.
+
+(*
+  def client() : 1 {
+    let server = new in
+    spawn server_init();
+    let self = new in
+    server!Connect[self];
+    guard self : _ {
+      receive Ack[r] from self |-> client_beat(self, r)
+    }
+  }
+
+  def client_beat(self, server) {
+    server!Beat[self];
+    guard self : _ {
+      receive Beat[r] from self |-> client_beat(self, r)
+      receive Close[r] from self |-> 
+    }
+  }
+*)
+(**)
+(*Section heartbeat.*)
+(**)
+(*  Inductive Heartbeat : Type :=*)
+(*    | StartHearbeat : Heartbeat*)
+(*    | Beat : Heartbeat*)
+(*    | Close : Heartbeat*)
+(*    | Ack : Heartbeat.*)
+(**)
+(*  Instance HeartbeatMessage : IMessage Heartbeat.*)
+(*  Proof.*)
+(*    constructor.*)
+(*    - destruct m, n; try (now left); try (now right).*)
+(*    - apply (fun _ => 1).*)
+(*  Defined.*)
+(**)
+(*  Definition StartHeartbeatType := ? (⋆ « Beat » ⊕ « Close »).*)
+(*  Definition BeatType := TTBase (BTUnit).*)
+(*  Definition CloseType := ? « Ack ».*)
+(*  Definition AckType := TTBase (BTUnit).*)
+(**)
+(*  Definition HeartbeatMessage_Types (m : Heartbeat) :=*)
+(*    match m with*)
+(*    | StartHearbeat => TTMailbox (? (⋆ « Beat » ⊕ « Close »))*)
+(*    | Close => TTMailbox (? « Ack »)*)
+(*    | _ => TTBase BTUnit*)
+(*    end.*)
+(**)
+(*End heartbeat.*)
+(**)
+(**)
+(*Section ping_pong_example.*)
+(**)
+(*  Inductive PingPong : Type :=*)
+(*    | Ping  : PingPong*)
+(*    | Pong  : PingPong*)
+(*    | Abort : PingPong*)
+(*    | Ack   : PingPong.*)
+(**)
+(*  Instance PingPongMessage : IMessage PingPong.*)
+(*  Proof.*)
+(*    constructor.*)
+(*    - destruct m, n; try (now left); try (now right).*)
+(*    - apply (fun _ => 1).*)
+(*  Defined.*)
+(**)
+(*  Definition PingType := ! « Pong ».*)
+(*  Definition PongType := TTBase (BTUnit).*)
+(*  Definition AbortType := ? «  ».*)
+(**)
+(*End ping_pong_example.*)
+(**)
 Section future_example.
 
 (** [Future] defines the message atoms *)
@@ -63,8 +580,8 @@ Definition FutureMessageTypes (m : Future) : list TType :=
     emptyFuture : EmptyFutureType -> 1
 *)
 Definition EmptyFutureBody : Term :=
-  TGuard (ValueVar (Var 0)) (« Put » ⊙ (⋆ « Get »)) [
-    GReceive Put (Var 0) (TApp FullFutureDef [ValueVar (Var 1) ; ValueVar (Var 0)])
+  TGuard (ValueVar 0) (« Put » ⊙ (⋆ « Get »)) [
+    GReceive Put (TValue (ValueVar 0)) (TApp FullFutureDef [ValueVar 1; ValueVar 0])
   ].
 
 Definition EmptyFuture : FunctionDefinition :=
